

PART A: NO CALCULATOR

1. Simplify:

a) $\frac{(10x^{\frac{5}{3}}y^{-5})(9x^{\frac{4}{3}}y^2)}{6xy^{-7}}$

$$= \frac{90x^3y^{-3}}{6xy^{-7}}$$

$$= 15x^2y^4$$

4

b) $\frac{5^{-4}+5^{-1}}{5^{-4}+5^{-2}}$

$$= \frac{5^{-4}(1+5^3)}{5^{-4}(1+5^2)}$$

$$= \frac{126}{26}$$

$$= \frac{63}{13}$$

2. Evaluate.

a) $\log_5 125$

$$= 3$$

b) $\log_9 3 + 2\log_9 3$

$$= 3\log_9 3$$

$$= 3\left(\frac{1}{2}\right)$$

$$= \frac{3}{2}$$

b) $\log_3(\sqrt{27} \cdot 9) + \log_4(8)$

$$= \log_3(3^{\frac{3}{2}} \cdot 3^2) + \log_4 8$$

$$= \log_3(3^{\frac{7}{2}}) + \log_4 8$$

$$= \frac{7}{2} + \frac{3}{2}$$

$$= 5$$

5

3. Rewrite in either exponential/logarithmic form.

a) $\log_d e = k$

$$\therefore d^k = e$$

b) $g^p = r$

$$\therefore \log_g r = p$$

2

4. Write as a single log:

$$\log_3 M + \log_3 N + \frac{1}{2}\log_3 P$$

$$= \log_3 MN + \log_3 P^{\frac{1}{2}}$$

$$= \log_3 MNP^{\frac{1}{2}}$$

4

5. Solve for exact value(s).

$$2\log_5 x = \log_5 50$$

$$\log_5 x^2 = \log_5 50$$

$$\therefore x^2 = 50$$

$$x = \pm\sqrt{50}$$

$$\rightarrow = \pm 5\sqrt{2}$$

inadmissible

Please raise your hand to hand in this section of your test and receive the next section.

PART B: CALCULATOR PERMITTED

Name: _____

1. Solve to exact value(s):

a) $2^{2x} - 4(2^x) = 32$

$$2^{2x} - 4(2^x) - 32 = 0$$

$$(2^x - 8)(2^x + 4) = 0$$

$$\therefore 2^x = 2^3 \quad \text{or} \quad 2^x = -4$$

$$\therefore x = 3 \quad \text{no sol'n}$$

b) $\log_2(x - 3) - \log_2(x + 1) = 3$

$$\log_2\left(\frac{x-3}{x+1}\right) = 3$$

$$\therefore \frac{x-3}{x+1} = 8$$

$$x-3 = 8x+8$$

$$-11 = 7x$$

inadmissible
 $x = -\frac{11}{7}$

\therefore No Solution

c) $\log_3(x + 5) + \log_3(x - 2) = 2\log_3 4$

$$\log_3(x^2 + 3x - 10) = \log_3 16$$

$$\therefore x^2 + 3x - 10 = 16$$

$$x^2 + 3x - 26 = 0$$

$$\therefore x = \frac{-3 \pm \sqrt{9 + 104}}{2}$$

$$= \frac{-3 \pm \sqrt{113}}{2}$$

inadmissible

d) $4^{x^2-3} = \left(\frac{1}{16}\right)^{5x+3} \times 64^{-2}$

$$4^{x^2-3} = (4^{-10x-6})(4^{-6})$$

$$4^{x^2-3} = 4^{-10x-12}$$

$$\therefore x^2 - 3 = -10x - 12$$

$$x^2 + 10x + 9 = 0$$

$$(x+9)(x+1) = 0$$

$$\therefore x = -9 \text{ or } -1$$

18

e) $5(3^{x-1}) = 4(27^x)$

$$\log[5(3^{x-1})] = \log[4(27^x)]$$

$$\log 5 + \log 3^{x-1} = \log 4 + \log 27^x$$

$$\log 5 + (x-1)\log 3 = \log 4 + x\log 27$$

$$\log 5 + x\log 3 - \log 3 = \log 4 + x\log 27$$

$$x(\log 3 - \log 27) = \log 4 - \log 5 + \log 3$$

$$x(-2\log 3) = -\log 5 + \log 4 + \log 3$$

$$x = \frac{\log 5 - \log 4 - \log 3}{2\log 3}$$

f) $2^{2x-1} + 2^{2x-5} = 272$

$$2^{2x-5}(2^4 + 1) = 272$$

$$2^{2x-5}(17) = 272$$

$$2^{2x-5} = 2^4$$

$$\therefore 2x - 5 = 4$$

$$x = \frac{9}{2}$$

2. Prove that $\frac{1}{\log_3 x} + \frac{2}{\log_4 x} + \frac{1}{\log_5 x} = \frac{1}{\log_{240} x}$

3

$$\begin{aligned} LS &= \log_x 3 + 2\log_x 4 + \log_x 5 \\ &= \log_x 15 + \log_x 16 \\ &= \log_x 240 \\ &= \frac{1}{\log_{240} x} \end{aligned}$$

3. If $\log_b x = 7$, find the value of $\log_b (x\sqrt{x})$

3

$$\begin{aligned} \textcircled{1} \quad \therefore b^7 &= x \\ \text{sub } \textcircled{1} \text{ in } \textcircled{2} \\ \therefore \log_b (b^7 \sqrt{b^7}) &= \log_b (b^7 \cdot b^{\frac{7}{2}}) \\ &= \log_b (b^{\frac{21}{2}}) \end{aligned}$$

$$\begin{aligned} \textcircled{2} \quad &= \log_b (b^{\frac{21}{2}}) \\ \therefore \frac{21}{2} &= \underline{\underline{21/2}} \end{aligned}$$

$$\begin{aligned} \log_b x + \log_b \sqrt{x} &= \log_b x + \frac{1}{2} \log_b x \\ &= 7 + \frac{7}{2} \\ &= \frac{21}{2} \end{aligned}$$

4. If $\log_b a = x^2$ and $\log_a b = \frac{9}{x^4}$, show that $x = \pm 3$.

$$\textcircled{1} \quad \therefore b^{x^2} = a \quad \textcircled{2} \quad \therefore a^{\frac{9}{x^4}} = b$$

sub $\textcircled{1}$ in $\textcircled{2}$

$$(b^{x^2})^{\frac{9}{x^4}} = b$$

$$b^{\frac{9}{x^2}} = b$$

$$\therefore \frac{9}{x^2} = 1$$

$$\begin{aligned} x^2 &= 9 \\ x &= \pm 3 \end{aligned}$$